work on funcall

Nelist.v
@@ -110,7 +110,7 @@ Inductive NoDup {A : Type} : nelist A -> Prop :=
     NoDup_base : forall x, NoDup (nebase x)
   | NoDup_cons : forall x l, ~In x l -> NoDup l -> NoDup (necons x l).
 
-Definition nefst {A B: Type} (l: nelist (A * B)): nelist A :=
+Definition map_fst {A B: Type} (l: nelist (A * B)): nelist A :=
   map (@fst A B) l.
 
 (** ** Properties *)
