Simu/Sem.v
@@ -163,7 +163,7 @@ with stmt_step_eval: program -> menv -> ident -> nelist val -> menv -> val -> Pr
      | Iestep:
          forall prog menv env clsid vs prog' S' rv cls,
            find_class clsid prog = Some (cls, prog') ->
-           env = adds (Nelist.nefst cls.(c_input)) vs v_empty ->
+           env = adds (Nelist.map_fst cls.(c_input)) vs v_empty ->
            stmt_eval prog' (menv, env) cls.(c_step) S' ->
            find_var (fst cls.(c_output)) S' rv ->
            stmt_step_eval prog menv clsid vs (fst S') rv.
@@ -237,6 +237,164 @@ Ltac app_stmt_eval_det :=
         H2: stmt_eval ?prog ?S ?s ?S2 |- _ =>
     let H := fresh in
     assert (S2 = S1) as H by (eapply stmt_eval_det; eauto); inverts H; clear H2
+  end.
+
+Inductive sub_prog: program -> program -> Prop :=
+  sub_prog_intro: forall p p',
+    sub_prog p (p' ++ p).
+
+Lemma find_class_sub:
+  forall prog clsid cls prog',
+    find_class clsid prog = Some (cls, prog') ->
+    sub_prog prog' prog.
+Proof.
+  introv Find.
+  forwards* (prog2' & ? & ?): find_class_app Find.
+  substs.
+  rewrite List_shift_first.
+  constructor.
+Qed.
+
+Hint Constructors sub_prog.
+
+Definition unique_classes (prog: program): Prop :=
+  forall c1 c2,
+    List.In c1 prog ->
+    List.In c2 prog ->
+    c1.(c_name) <> c2.(c_name).
+
+Remark unique_nil :
+  unique_classes nil.
+Proof.
+  unfold unique_classes; intros; contradiction.
+Qed.
+
+Remark unique_cons:
+  forall cls c,
+    unique_classes (c :: cls) -> unique_classes cls.
+Proof.
+  destruct cls.
+  - intros; apply unique_nil.
+  - intros c' H.
+    unfold unique_classes.
+    introv Hin1 Hin2.
+    unfold unique_classes in H.
+    apply List.in_cons with (a:=c') in Hin1.
+    apply List.in_cons with (a:=c') in Hin2.
+    specializes H Hin1 Hin2.
+Qed.
+
+Remark unique_app:
+  forall cls cls',
+    unique_classes (cls ++ cls') -> unique_classes cls /\ unique_classes cls'.
+Proof.
+  induction cls.
+  - simpl; split; auto. apply unique_nil.
+  - intros cls' Unique.
+    split.
+    + unfold unique_classes.
+      introv Hin1 Hin2.
+      unfold unique_classes in Unique.
+      apply Unique; apply List.in_or_app; left; auto.
+    + rewrite <-List.app_comm_cons in Unique.  
+      apply unique_cons in Unique.
+      apply IHcls; auto.
+Qed.
+
+Remark find_class_sub_same:
+  forall prog1 prog2 clsid cls prog',
+    find_class clsid prog2 = Some (cls, prog') ->
+    unique_classes prog1 ->
+    sub_prog prog2 prog1 ->
+    find_class clsid prog1 = Some (cls, prog').
+Proof.
+  introv Hfind Unique Sub.
+  inverts Sub.
+  forwards* (prog2' & Hprog2 & Hnone): find_class_app Hfind.
+  induction p'; simpl; auto.
+  rewrite <-List.app_comm_cons in Unique.
+  assert (List.In a (a :: p' ++ prog2)) as Hin_a by apply List.in_eq.
+  assert (List.In cls (a :: p' ++ prog2)) as Hin_cls.
+  - forwards* Hin: find_class_In Hfind.
+    rewrite List.app_comm_cons.   
+    apply List.in_or_app; right; auto. 
+  - forwards Neq: Unique Hin_a Hin_cls.
+    apply ident_eqb_neq in Neq.
+    forwards* Eq: find_class_name Hfind.
+    rewrite Eq in Neq; rewrite Neq.
+    apply IHp'. eapply unique_cons; eauto.
+Qed.
+
+Remark find_class_unique:
+  forall prog clsid cls prog',
+    unique_classes prog ->
+    find_class clsid prog = Some (cls, prog') ->
+    unique_classes prog'.
+Proof.
+  introv Unique Find.
+  forwards* (prog2' & Hprog2 & Hnone): find_class_app Find.
+  substs.
+  forwards (? & H): unique_app Unique.
+  eapply unique_cons; eauto.
+Qed.
+
+Lemma stmt_step_eval_det':
+  forall prog1 prog2 me clsid vs me1 rv1 me2 rv2,
+    unique_classes prog1 ->
+    stmt_step_eval prog1 me clsid vs me1 rv1 ->
+    stmt_step_eval prog2 me clsid vs me2 rv2 ->
+    sub_prog prog2 prog1 ->
+    me1 = me2 /\ rv1 = rv2.
+Proof.
+  introv Unique Hstp1; revert me2 rv2 prog2.
+  induction Hstp1 using stmt_step_eval_ind_2 with
+  (P := fun p S s S' => unique_classes p -> forall S'', stmt_eval p S s S' -> stmt_eval p S s S'' -> S' = S'');
+    [| | | | | |introv Hstp2 Hsub]; try (introv Hev1 Hev2; inverts Hev2); try app_exp_eval_det; auto. 
+  - app_bool_val; auto.
+  - apply* IHHstp0.
+    asserts_rewrite* (S2 = S4).
+  - assert (omenv = omenv0) by apply* find_inst_det; subst omenv0.
+    assert (vs = vs0) by (eapply Forall2_det; eauto; eapply exp_eval_det); subst vs0.
+    repeat fequals; apply* IHHstp1;
+    rewrite* <-List.app_nil_l; simpl.
+  - inverts Hstp2.
+    substs.
+    forwards* H': find_class_sub_same.
+    rewrite H' in H; inverts H.
+    forwards Unique': find_class_unique Unique H'.
+    assert (S' = S'0); auto. subst S'0.
+    split*.
+    apply* find_var_det.
+Qed.
+
+Theorem stmt_eval_det':
+  forall prog1 prog2 S s S1 S2,
+    unique_classes prog1 ->
+    stmt_eval prog1 S s S1 ->
+    stmt_eval prog2 S s S2 ->
+    sub_prog prog2 prog1 ->
+    S1 = S2.
+Proof.
+  intros until S2; intros Unique Hev1; revert S2;
+  induction Hev1; intros S2' Hev2 Hsub; inv Hev2; inv Hsub;
+  try app_exp_eval_det; auto.
+  - apply* IHHev1.
+    app_bool_val; eauto.    
+  - apply* IHHev1_2.
+    asserts_rewrite* (S2 = S4).
+  - assert (omenv = omenv0) by apply* find_inst_det; subst omenv0.
+    assert (vs = vs0) by (eapply Forall2_det; eauto; eapply exp_eval_det); subst vs0.
+    repeat fequals; apply* stmt_step_eval_det'.
+Qed.
+
+Ltac app_stmt_eval_det' :=
+  match goal with
+  | H1: stmt_eval ?prog1 ?S ?s ?S1,
+        H2: stmt_eval ?prog2 ?S ?s ?S2,
+            H3: sub_prog ?prog2 ?prog1,
+                H4: unique_classes ?prog1 |- _ =>
+    let H := fresh in
+    assert (S1 = S2) as H by (applys stmt_eval_det' H4 H1 H2 H3; eauto); inverts H; clear H2
   end.
 
 (* Inductive cont := *)
